examples/security/statefulEnc-multi-hyperheap.fst
@@ -1,0 +1,236 @@
+(*--build-config
+    options:--admit_fsi Set --admit_fsi Seq --admit_fsi Map;
+    other-files:../../lib/ext.fst ../../lib/set.fsi ../../lib/heap.fst ../../lib/map.fsi ../../lib/hyperheap.fst ../../lib/seq.fsi
+  --*)
+(* A standalone experiment corresponding to building a stateful encryption on
+   top of a stateless one ... along the lines of StatefulLHAE on top of AEAD_GCM *)
+
+(* Still to do:
+     Show that multiple instances do not overlap using footprints and dynamic frames
+*)
+module StatefulEncryption.MultiInstance.HyperHeap
+open ST
+open Set
+open Seq
+open HyperHeap
+
+(* TODO: merge these next two functions and lemma/assumption with the seq library *)
+val snoc : seq 'a -> 'a -> Tot (seq 'a)
+let snoc s x = Seq.append s (Seq.create 1 x)
+
+assume val emp: #a:Type -> Tot (seq a)
+assume Length_emp: forall (a:Type).{:pattern (Seq.length (emp #a))} Seq.length (emp #a) = 0
+
+//type Fresh (#a:Type) h0 (r:ref a) h1 = Heap.contains h1 r /\ not (Heap.contains h0 r)
+
+type Let (#a:Type) (x:a) (body: (y:a{y=x} -> Type)) = body x
+
+type plain
+type cipher
+type key
+
+type basicEntry =
+  | Entry : p:plain -> c:cipher -> basicEntry
+
+type encryptor (i:rid) =
+  | Enc : log:rref i (seq basicEntry) -> key -> encryptor i
+
+type decryptor (i:rid) =
+  | Dec : log:rref i (seq basicEntry) -> key -> decryptor i
+
+type paired (#i:rid) (e:encryptor i) (d:decryptor i) = b2t (Enc.log e = Dec.log d)
+
+type both =
+  | Both : i:rid -> e:encryptor i -> d:decryptor i{paired e d} -> both
+
+type Fresh (#a:Type) h0 (r:ref a) h1 = Heap.contains h1 r /\ not (Heap.contains h0 r)
+
+val gen: unit -> ST both
+  (requires (fun h -> True))
+  (ensures (fun h0 b h1 ->
+      modifies Set.empty h0 h1
+      /\ not (Map.contains h0 (Both.i b))
+      /\ Map.contains h1 (Both.i b)
+      /\ Heap.contains (Map.sel h1 (Both.i b))
+                       (as_ref (Enc.log (Both.e b)))
+      /\ sel h1 (Enc.log (Both.e b)) = emp))
+let gen () =
+  let key : key = magic () in
+  let region = new_region () in
+  let log = ralloc region emp in
+  Both region (Enc log key) (Dec log key)
+
+opaque logic type modifies (mods:set Heap.aref) (h:heap) (h':heap) =
+    b2t (Heap.equal h' (Heap.concat h' (Heap.restrict h (complement mods))))
+
+val enc : #i:rid -> e:encryptor i -> p:plain -> ST cipher
+    (requires (fun h -> True))
+    (ensures (fun h0 c h1 ->
+                HyperHeap.modifies (Set.singleton i) h0 h1
+                /\ modifies !{as_ref (Enc.log e)} (Map.sel h0 i) (Map.sel h1 i)
+                /\ h1 = upd h0 (Enc.log e) (snoc (sel h0 (Enc.log e)) (Entry p c))))
+let enc i e p =
+    let c : cipher = magic () in
+    op_ColonEquals (Enc.log e) (snoc (op_Bang (Enc.log e)) (Entry p c));
+    c
+
+assume val find_seq : #a:Type -> f:(a -> Tot bool) -> s:seq a
+            -> Tot (o:option (i:nat{i < Seq.length s /\ f (Seq.index s i)}) { is_None o ==> (forall (i:nat{i < Seq.length s}). not (f (Seq.index s i)))})
+
+opaque logic type trigger (i:nat) = True
+val dec: #i:rid -> d:decryptor i -> c:cipher -> ST (option plain)
+  (requires (fun h -> True))
+  (ensures (fun h0 p h1 ->
+              HyperHeap.modifies Set.empty h0 h1
+              /\ (Let (sel h0 (Dec.log d))
+                      (fun log ->
+                          (is_None p ==> (forall (i:nat{i < Seq.length log}). Entry.c (Seq.index log i) <> c))
+                          /\ (is_Some p ==> (exists (i:nat{i < Seq.length log}).{:pattern (trigger i)} Seq.index log i = Entry (Some.v p) c))))))
+let dec i d c =
+  let s = op_Bang (Dec.log d) in
+  match find_seq (function Entry p c' -> c=c') s with
+    | None -> None
+    | Some j -> cut (trigger j); Some (Entry.p (Seq.index s j))
+
+(* -------------------------------------------------------- *)
+type statefulEntry =
+  | StEntry : i:nat -> p:plain -> c:cipher -> statefulEntry
+
+type st_encryptor (i:rid) =
+  | StEnc : log: rref i (seq statefulEntry) -> ctr: rref i nat -> key:encryptor i -> st_encryptor i
+
+type st_decryptor (i:rid) =
+  | StDec : log: rref i (seq statefulEntry) -> ctr: rref i nat -> key:decryptor i -> st_decryptor i
+
+type st_paired (#i:rid) (enc:st_encryptor i) (dec:st_decryptor i) =
+      StEnc.log enc = StDec.log dec
+      /\ paired (StEnc.key enc) (StDec.key dec)
+      /\ as_ref (Enc.log (StEnc.key enc)) =!= as_ref (StEnc.log enc)
+      /\ as_ref (StEnc.ctr enc) <> as_ref (StDec.ctr dec)
+      /\ as_ref (StEnc.log enc) =!= as_ref (StEnc.ctr enc)                      //These last four are needed because seq is abstract
+      /\ as_ref (StEnc.log enc) =!= as_ref (StDec.ctr dec)                      //...
+      /\ as_ref (Enc.log (StEnc.key enc)) =!= as_ref (StEnc.ctr enc)            //...
+      /\ as_ref (Enc.log (StEnc.key enc)) =!= as_ref (StDec.ctr dec)            //and so potentially equal to nat ... TODO: make seq a new type
+
+type st_both =
+  | STBoth : i:rid -> e:st_encryptor i -> d:st_decryptor i{st_paired e d} -> st_both
+
+assume val with_seqn : nat -> plain -> Tot plain
+
+type st_inv (#i:rid) (e:st_encryptor i) (d:st_decryptor i) (h:HyperHeap.t) =
+  st_paired e d
+  /\ Map.contains h i
+  /\ Heap.contains (Map.sel h i) (as_ref (StEnc.log e))
+  /\ Heap.contains (Map.sel h i) (as_ref (StEnc.ctr e))
+  /\ Heap.contains (Map.sel h i) (as_ref (StDec.ctr d))
+  /\ Heap.contains (Map.sel h i) (as_ref (Enc.log (StEnc.key e)))
+  /\ Let (sel h (Enc.log (StEnc.key e))) (fun basic ->
+     Let (sel h (StEnc.log e)) (fun st ->
+     Let (sel h (StEnc.ctr e)) (fun w ->
+     Let (sel h (StDec.ctr d)) (fun r ->
+     Seq.length st = Seq.length basic
+     /\ w = Seq.length st
+     /\ r <= w
+     /\ (forall (i:nat{i < Seq.length st}).
+          Let (Seq.index st i) (fun st_en ->
+            StEntry.i st_en = i
+            /\ Seq.index basic i = Entry (with_seqn i (StEntry.p st_en)) (StEntry.c st_en)))))))
+
+type st_enc_inv (#i:rid) (e:st_encryptor i) (h:HyperHeap.t) =
+  exists (d:st_decryptor i). st_inv e d h
+
+type st_dec_inv (#i:rid) (d:st_decryptor i) (h:HyperHeap.t) =
+  exists (e:st_encryptor i). st_inv e d h
+
+let refs_in_e (#i:rid) (e:st_encryptor i) = !{as_ref (StEnc.log e), as_ref (StEnc.ctr e), as_ref (Enc.log (StEnc.key e))}
+let refs_in_d (#i:rid) (d:st_decryptor i) = !{as_ref (StDec.log d), as_ref (StDec.ctr d), as_ref (Dec.log (StDec.key d))}
+
+val stateful_gen : unit -> ST st_both
+  (requires (fun h -> True))
+  (ensures (fun h0 b h1 ->
+              st_inv (STBoth.e b) (STBoth.d b) h1
+              /\ HyperHeap.modifies Set.empty h0 h1
+              /\ not (Map.contains h0 (STBoth.i b))
+              /\ Map.contains h1 (STBoth.i b)))
+let stateful_gen () =
+  let Both i e d = gen () in
+  let l = ralloc i emp in
+  let w = ralloc i 0 in
+  let r = ralloc i 0 in
+  STBoth i (StEnc l w e) (StDec l r d)
+
+val stateful_enc : #i:rid -> e:st_encryptor i -> p:plain -> ST cipher
+  (requires (fun h -> st_enc_inv e h))
+  (ensures (fun h0 c h1 ->
+                    st_enc_inv e h1
+                 /\ HyperHeap.modifies (Set.singleton i) h0 h1
+                 /\ modifies (refs_in_e e) (Map.sel h0 i) (Map.sel h1 i)
+                 /\ sel h1 (StEnc.log e) = snoc (sel h0 (StEnc.log e)) (StEntry (sel h0 (StEnc.ctr e)) p c)))
+let stateful_enc i e p =
+  let i = op_Bang (StEnc.ctr e) in
+  let ip = with_seqn i p in
+  let c = enc (StEnc.key e) ip in
+  op_ColonEquals (StEnc.log e) (snoc (op_Bang (StEnc.log e)) (StEntry i p c));
+  op_ColonEquals (StEnc.ctr e) (i + 1);
+  c
+
+val stateful_dec: #i:rid -> ad:nat -> d:st_decryptor i -> c:cipher -> ST (option plain)
+  (requires (fun h -> st_dec_inv d h))
+  (ensures (fun h0 p h1 ->
+                st_dec_inv d h0
+                /\ st_dec_inv d h1
+                /\ HyperHeap.modifies (Set.singleton i) h0 h1
+                /\ modifies !{as_ref (StDec.ctr d)} (Map.sel h0 i) (Map.sel h1 i)
+                /\ Let (sel h0 (StDec.ctr d)) (fun (r:nat{r=sel h0 (StDec.ctr d)}) ->
+                   Let (sel h0 (StDec.log d)) (fun (log:seq statefulEntry{log=sel h0 (StDec.log d)}) ->
+                    (is_None p ==> (r = Seq.length log                     //nothing encrypted yet
+                                    || StEntry.c (Seq.index log r) <> c    //bogus cipher
+                                    || r <> ad))                           //reading at the wrong postition
+                   /\ (is_Some p ==>
+                          ((sel h1 (StDec.ctr d) = r + 1)
+                           /\ StEntry.p (Seq.index log r) = Some.v p))))))
+let stateful_dec i ad d c =
+  match dec (StDec.key d) c with
+    | None -> None
+    | Some p ->
+      let i = op_Bang (StDec.ctr d) in
+      let l = op_Bang (StDec.log d) in
+      if i < Seq.length l
+      then let StEntry _ q _ = Seq.index l i in
+           if i = ad
+           then (op_ColonEquals (StDec.ctr d) (i + 1); Some q)
+           else None
+      else None
+
+
+val test_st_frame : #i:rid -> #j:rid{i<>j}
+                   -> s1:st_both{STBoth.i s1 = i}
+                   -> s2:st_both{STBoth.i s2 = j}
+                   -> ST unit
+  (requires (fun h ->
+                 st_inv (STBoth.e s1) (STBoth.d s1) h
+              /\ st_inv (STBoth.e s2) (STBoth.d s2) h
+              /\ sel h (StEnc.ctr (STBoth.e s1)) = sel h (StDec.ctr (STBoth.d s1))
+              // /\ Heap.sel h (StEnc.ctr (STI.e s2)) = Heap.sel h (StDec.ctr (STI.d s2))
+              ))
+  (ensures (fun h0 _ h1 ->
+                 st_inv (STBoth.e s1) (STBoth.d s1) h1
+              /\ st_inv (STBoth.e s2) (STBoth.d s2) h1
+              /\ HyperHeap.modifies (Set.union (Set.singleton i) (Set.singleton j)) h0 h1))
+// note that we do not require new encryptor/decryptors,
+// just that those in s1 are in sync, so that decryption cancels encryption
+assume val mk_plain : unit -> ST plain (requires (fun h -> True)) (ensures (fun h0 x h1 -> h0=h1))
+let test_st_frame i j s1 s2 =
+  let p = mk_plain () in
+  let q = mk_plain () in
+  let g = stateful_gen () in
+  // let s3 = stateful_gen() // also type-breaking; yes, because this modifies fp, basic_fp
+  let ctr = op_Bang (StEnc.ctr (STBoth.e s1)) in
+  let c0 = stateful_enc (STBoth.e s1) p in
+  let c1 = stateful_enc (STBoth.e s1) q in
+  let c2 = stateful_enc (STBoth.e s2) p in
+  // let oX = stateful_dec (STBoth.d s1) c2 in // might succeed
+  let o0 = stateful_dec (ctr) (STBoth.d s1) c0 in
+  let o1 = stateful_dec (ctr + 1) (STBoth.d s1) c1 in
+  assert (Some.v o0 = p);
+  assert (Some.v o1 = q)
