examples/unit-tests/testhyperheap.fst
@@ -8,7 +8,7 @@ open HyperHeap
 
 val test0: #r:rid -> i:int -> v:rref r int -> ST int
   (requires (fun m0 -> Map.contains m0 r))
-  (ensures (fun m0 k m1 -> k=i+(Heap.sel (Map.sel m0 r) (as_ref v))
+  (ensures (fun m0 k m1 -> k=i+sel m0 v
                         /\ modifies Set.empty m0 m1))
 let test0 _r i v =
   let r = new_region () in
